tests/lean/Hashmap/FunsExternal.lean
@@ -1,0 +1,19 @@
+-- [hashmap]: external functions.
+import Base
+import Hashmap.Types
+open Primitives
+open hashmap
+
+-- TODO: fill those bodies
+
+/- [hashmap::hashmap_utils::deserialize]:
+   Source: 'tests/src/hashmap.rs', lines 330:4-330:47 -/
+def hashmap_utils.deserialize
+  : State → Result (State × (HashMap U64)) :=
+  fun _ => .fail .panic
+
+/- [hashmap::hashmap_utils::serialize]:
+   Source: 'tests/src/hashmap.rs', lines 325:4-325:46 -/
+def hashmap_utils.serialize
+  : HashMap U64 → State → Result (State × Unit) :=
+  fun _ _ => .fail .panic
